compiler/proof_vec/new_test_proof.ec
@@ -1,12 +1,21 @@
-require import Int IntDiv Jasmin_model Gimli_ref Gimli_ref1 Gimliv CoreMap.
+require import AllCore Jasmin_model Gimli_ref Gimli_ref1 Gimliv1 Gimliv CoreMap.
+
+
+hint simplify pow_le0.
+hint simplify powS_minus@1.
+hint simplify (pow2_1, pow2_2, pow2_3, pow2_4, pow2_5, pow2_6, pow2_7, pow2_8)@0.
+
+hint simplify (W8.of_uintK, W8.to_uintK', W32.of_uintK, W32.to_uintK')@0.
+hint simplify (pack_unpack_4u32, unpack_pack_4u32)@0.
+hint simplify (VPAND_128_32, VPOR_128_32, VPXOR_128_32)@0.
 
 axiom rol32_xor (x:W32.t) i : 0 <= i < 32 => 
  (x86_ROL_32 x ((of_int i)%W8)).`3  = (x `<<` (W8.of_int i)) `^` (x `>>` (W8.of_int (32 - i))).
 
 equiv rotate_ref_ref1 : Gimli_ref.M.rotate ~ Gimli_ref1.M.rotate : ={x,bits} /\ 0 <= bits{1} < 32 ==> ={res}.
 proof.
-by proc;auto => &m1 &m2 /> ??;apply (rol32_xor x{m2} bits{m2}). qed. 
-
+ by proc;auto => &m1 &m2 /> ??; apply (rol32_xor x{m2} bits{m2}). 
+qed. 
 
 equiv Gimli_ref_ref1 : Gimli_ref.M.gimli_body ~ Gimli_ref1.M.gimli_body : ={state} ==> ={res}.
 proof.
@@ -16,85 +25,72 @@ proof.
   sim; do 2! (call rotate_ref_ref1; sim />).
 qed.
 
-op of32 : W32.t -> W32.t -> W32.t -> W32.t -> W128.t.
-op to32 : W128.t -> W32.t -> W32.t -> W32.t.
+axiom xor_zero_l x : W32.zeros `^` x = x.
+axiom xor_zero_r x : x `^` W32.zeros = x.
 
-op zero   : W32.t.
-
-axiom xor_zero_l x : zero `^` x = x.
-axiom xor_zero_r x : x `^` zero = x.
-
-axiom of32_shl x0 x1 x2 x3 i: 
-  (of32 x0 x1 x2 x3) `<<` i = 
-  of32 (x0 `<<` i) (x1 `<<` i) (x2 `<<` i) (x3 `<<` i).
-
-axiom of32_shr x0 x1 x2 x3 i: 
-  of32 x0 x1 x2 x3 `>>` i = 
-  of32 (x0 `>>` i) (x1 `>>` i) (x2 `>>` i) (x3 `>>` i).
-
-axiom of32_xor x0 x1 x2 x3 y0 y1 y2 y3 : 
-  of32 x0 x1 x2 x3 `^` of32 y0 y1 y2 y3 = 
-  of32 (x0 `^` y0) (x1 `^` y1) (x2 `^` y2) (x3 `^` y3).
-
-axiom of32_and x0 x1 x2 x3 y0 y1 y2 y3 : 
-  of32 x0 x1 x2 x3 `&` of32 y0 y1 y2 y3 = 
-  of32 (x0 `&` y0) (x1 `&` y1) (x2 `&` y2) (x3 `&` y3).
-
-axiom of32_or x0 x1 x2 x3 y0 y1 y2 y3 : 
-  of32 x0 x1 x2 x3 `|` of32 y0 y1 y2 y3 = 
-  of32 (x0 `|` y0) (x1 `|` y1) (x2 `|` y2) (x3 `|` y3).
-
-axiom shuffle4_u32_2301 x0 x1 x2 x3 : 
-  x86_VPSHUFD_128 (of32 x0 x1 x2 x3) (W8.of_int 177) (*shuffle 2 3 0 1*) = 
-  of32 x1 x0 x3 x2.
-
-axiom shuffle4_u32_1032 x0 x1 x2 x3 : 
-  x86_VPSHUFD_128 (of32 x0 x1 x2 x3) (W8.of_int 78) (*shuffle 1 0 3 2*) = 
-  of32 x2 x3 x0 x1.
-
-axiom of32_x86_VPSLL x0 x1 x2 x3 i :
-  x86_VPSLL_4u32 (of32 x0 x1 x2 x3) i =
-  of32 (x0 `<<` i) (x1 `<<` i) (x2 `<<` i) (x3 `<<` i).
-
-axiom of32_x86_VPSRL x0 x1 x2 x3 i :
-  x86_VPSRL_4u32 (of32 x0 x1 x2 x3) i =
-  of32 (x0 `>>` i) (x1 `>>` i) (x2 `>>` i) (x3 `>>` i).
+hint simplify (xor_zero_l, xor_zero_r)@0.
 
 axiom rotate24E w :
     x86_VPSHUFB_128  w (W128.of_int 16028905388486802350658220295983399425)
-  = ((w `<<` (W8.of_int 24)) `^` (w `>>` (W8.of_int 8))).
+  = x86_VPSLL_4u32 w (W8.of_int 24) `^` x86_VPSRL_4u32 w (W8.of_int 8).
 
 hint simplify xor_zero_l.
 hint simplify xor_zero_r.
-hint simplify of32_shl.
-hint simplify of32_shr.
-hint simplify of32_xor.
-hint simplify of32_and.
-hint simplify of32_or.
-(*hint simplify shuffle4_u32_2301.
-hint simplify shuffle4_u32_1032.*)
-hint simplify of32_x86_VPSLL.
-hint simplify of32_x86_VPSRL.
 hint simplify rotate24E.
 
-equiv ref1_vec1 : Gimli_ref1.M.gimli_body ~ Gimliv.M.gimli_body : 
-   (of32 state.[0] state.[1] state.[2]  state.[3] ){1} = x{2} /\
-   (of32 state.[4] state.[5] state.[6]  state.[7] ){1} = y{2} /\
-   (of32 state.[8] state.[9] state.[10] state.[11]){1} = z{2} 
+equiv ref1_vec1 : Gimli_ref1.M.gimli_body ~ Gimliv1.M.gimli_body1 : 
+   pack_4u32 (state.[0], state.[1], state.[2] , state.[3] ){1} = x{2} /\
+   pack_4u32 (state.[4], state.[5], state.[6] , state.[7] ){1} = y{2} /\
+   pack_4u32 (state.[8], state.[9], state.[10], state.[11]){1} = z{2} 
    ==>
-   (of32 res.[0] res.[1] res.[2]  res.[3] ){1} = res.`1{2} /\
-   (of32 res.[4] res.[5] res.[6]  res.[7] ){1} = res.`2{2} /\
-   (of32 res.[8] res.[9] res.[10] res.[11]){1} = res.`3{2}.
+   pack_4u32 (res.[0], res.[1], res.[2] , res.[3] ){1} = res.`1{2} /\
+   pack_4u32 (res.[4], res.[5], res.[6] , res.[7] ){1} = res.`2{2} /\
+   pack_4u32 (res.[8], res.[9], res.[10], res.[11]){1} = res.`3{2}.
 proof.
   proc; inline * => /=.
   while (#pre /\ ={round}); last by auto.
   unroll for {1} 2.
   wp; skip => &m1 &m2 [#].
   cbv delta => 4!<- _ _; cbv delta => />.
-split; move => h1.
-rewrite h1. split. auto.
-move => _.
-+ rewrite shuffle4_u32_2301.
-  admit.
-+ by rewrite shuffle4_u32_1032.
+qed.
+
+equiv vec1_vec : Gimliv1.M.gimli_body1 ~ Gimliv.M.gimli_body : 
+   ={x,y,z} ==> ={res}.
+proof.
+  proc. sim (_:true).
+  proc => /=; inline *;wp;skip => />.
+qed.
+
+equiv ref_vec : Gimli_ref.M.gimli_body ~ Gimliv.M.gimli_body : 
+   pack_4u32 (state.[0], state.[1], state.[2] , state.[3] ){1} = x{2} /\
+   pack_4u32 (state.[4], state.[5], state.[6] , state.[7] ){1} = y{2} /\
+   pack_4u32 (state.[8], state.[9], state.[10], state.[11]){1} = z{2} 
+   ==>
+   pack_4u32 (res.[0], res.[1], res.[2] , res.[3] ){1} = res.`1{2} /\
+   pack_4u32 (res.[4], res.[5], res.[6] , res.[7] ){1} = res.`2{2} /\
+   pack_4u32 (res.[8], res.[9], res.[10], res.[11]){1} = res.`3{2}.
+proof.
+  transitivity Gimli_ref1.M.gimli_body 
+    (={state} ==> ={res})
+    (pack_4u32 (state.[0], state.[1], state.[2] , state.[3] ){1} = x{2} /\
+   pack_4u32 (state.[4], state.[5], state.[6] , state.[7] ){1} = y{2} /\
+   pack_4u32 (state.[8], state.[9], state.[10], state.[11]){1} = z{2} 
+   ==>
+   pack_4u32 (res.[0], res.[1], res.[2] , res.[3] ){1} = res.`1{2} /\
+   pack_4u32 (res.[4], res.[5], res.[6] , res.[7] ){1} = res.`2{2} /\
+   pack_4u32 (res.[8], res.[9], res.[10], res.[11]){1} = res.`3{2}) => //.
+  + by move=> &m1 &m2 [#]???; exists state{m1}.  
+  by apply Gimli_ref_ref1.
+  transitivity Gimliv1.M.gimli_body1
+   (pack_4u32 (state.[0], state.[1], state.[2] , state.[3] ){1} = x{2} /\
+   pack_4u32 (state.[4], state.[5], state.[6] , state.[7] ){1} = y{2} /\
+   pack_4u32 (state.[8], state.[9], state.[10], state.[11]){1} = z{2} 
+   ==>
+   pack_4u32 (res.[0], res.[1], res.[2] , res.[3] ){1} = res.`1{2} /\
+   pack_4u32 (res.[4], res.[5], res.[6] , res.[7] ){1} = res.`2{2} /\
+   pack_4u32 (res.[8], res.[9], res.[10], res.[11]){1} = res.`3{2})
+   (={x,y,z} ==> ={res}) => //.
+  + by move=> &m1 &m2 [#]???; exists (x,y,z){m2}.
+  + by apply ref1_vec1.
+  by apply vec1_vec.   
 qed.
